ver2/symbolic_state_eval.v
@@ -33,39 +33,6 @@ Import EvalCommon.
 Module SymbolicStateEval.
 
 
-Inductive follow_in_smap_ret_t :=
-| FollowSmapVal (smv : smap_value) (key: nat) (sb: sbindings).
-
-
-Definition is_fresh_var_smv (smv: smap_value) :=
-  match smv with
-  | SymBasicVal (FreshVar idx) => Some idx
-  | _ => None
-  end.
-
-Definition not_basic_value_smv (smv: smap_value) :=
-  match smv with
-  | SymBasicVal _ => false
-  | _ => true
-  end.
-
-Fixpoint follow_in_smap (sv: sstack_val) (maxidx: nat) (sb: sbindings) : option follow_in_smap_ret_t :=
-  match sv with
-  | Val v => Some (FollowSmapVal (SymBasicVal (Val v)) maxidx sb)
-  | InStackVar n => Some (FollowSmapVal (SymBasicVal (InStackVar n)) maxidx sb)
-  | FreshVar idx =>
-      match sb with
-      | [] => None
-      | (key,smv)::sb' =>
-          if key =? idx then
-            match is_fresh_var_smv smv with
-            | Some idx' => follow_in_smap (FreshVar idx') key sb'
-            | Node => Some (FollowSmapVal smv key sb')
-            end
-          else follow_in_smap sv key sb'
-      end
-  end.
-
 
 Fixpoint eval_sstack_val' (d : nat) (sv : sstack_val) (stk : stack) (mem: memory) (strg: storage) (ctx: context) (maxidx: nat) (sb: sbindings) (ops: stack_op_instr_map) : option EVMWord :=
   match d with
